### 3-3

> 已知 $\gamma_5\equiv \gamma_1\gamma_2\gamma_3\gamma_4 $，证明：$\displaystyle{\gamma_5=\frac{1 }{4! } \varepsilon_{\mu\nu\alpha\beta}\gamma_\mu\gamma_\nu\gamma_\alpha\gamma_\beta }$ 

$$
\gamma_5
\equiv \gamma_1 \gamma_2 \gamma_3 \gamma_4
$$

上式两边同乘 $\varepsilon_{\mu\nu\lambda\rho} $：

$$
\begin{aligned}
\varepsilon_{\mu\nu\lambda\rho}\gamma_5
&=\varepsilon_{\mu\nu\lambda\rho} \gamma_1 \gamma_2 \gamma_3 \gamma_4 \\
&=\gamma_\mu \gamma_\nu \gamma_\lambda \gamma_\rho \\
\end{aligned}
$$

上式继续两边同乘 $\varepsilon_{\mu\nu\lambda\rho} $：

$$
\varepsilon_{\mu\nu\lambda\rho}\varepsilon_{\mu\nu\lambda\rho}\gamma_5
=\varepsilon_{\mu\nu\lambda\rho} \gamma_\mu \gamma_\nu \gamma_\lambda \gamma_\rho
$$

利用 $\varepsilon_{\mu\nu\lambda\rho}\varepsilon_{\mu\nu\lambda\rho}=4! $：

$$
4! \gamma_5
=\varepsilon_{\mu\nu\lambda\rho} \gamma_\mu \gamma_\nu \gamma_\lambda \gamma_\rho
$$

即：

$$
\gamma_5
=\frac{1 }{4! } \varepsilon_{\mu\nu\lambda\rho}  \gamma_\mu \gamma_\nu \gamma_\lambda \gamma_\rho
$$
